- A little more work on alphabetised predicates - Respinning introductory material in paper into (5) points

theories/theories/utp_designs_a.thy
@@ -2,6 +2,21 @@ theory utp_designs_a
 imports utp_designs
 begin
 
+definition DESIGN_ALPHABET :: "'a ALPHABET set" where
+"DESIGN_ALPHABET = {a \<in> REL_ALPHABET. \<lbrace>okay\<down>, okay\<down>\<acute>\<rbrace> \<subseteq>\<^sub>f a}"
+
+lemma REL_ALPHABET_DESIGN_ALPHABET [closure]:
+  "a \<in> DESIGN_ALPHABET \<Longrightarrow> a \<in> REL_ALPHABET"
+  by (simp add:DESIGN_ALPHABET_def)
+
+lemma DESIGN_ALPHABET_ok [closure]:
+  "a \<in> DESIGN_ALPHABET \<Longrightarrow> okay\<down> \<in> \<langle>a\<rangle>\<^sub>f"
+  by (auto simp add:DESIGN_ALPHABET_def)
+
+lemma DESIGN_ALPHABET_ok' [closure]:
+  "a \<in> DESIGN_ALPHABET \<Longrightarrow> okay\<down>\<acute> \<in> \<langle>a\<rangle>\<^sub>f"
+  by (auto simp add:DESIGN_ALPHABET_def)
+
 lift_definition DesignA :: 
   "'a WF_ALPHA_PREDICATE \<Rightarrow> 
    'a WF_ALPHA_PREDICATE \<Rightarrow> 
@@ -11,13 +26,31 @@ is "\<lambda> P Q. (\<alpha> P \<union>\<^sub>f \<alpha> Q \<union>\<^sub>f \<lb
   apply (auto intro:unrest)
 done
 
+definition SkipDA :: "'a ALPHABET \<Rightarrow> 'a WF_ALPHA_PREDICATE" where
+"SkipDA a = true\<^bsub>a\<^esub> \<turnstile>\<^sub>\<alpha> II\<alpha>\<^bsub>a -\<^sub>f \<lbrace>okay\<down>, okay\<down>\<acute>\<rbrace>\<^esub>"
+
+notation SkipDA ("II\<^bsub>D[_]\<^esub>")
+
+lift_definition AH1 :: 
+  "'a WF_ALPHA_PREDICATE \<Rightarrow> 
+   'a WF_ALPHA_PREDICATE"
+is "\<lambda> P. (\<alpha> P \<union>\<^sub>f \<lbrace>okay\<down>, okay\<down>\<acute>\<rbrace>, H1(\<pi> P))"
+  apply (simp add:WF_ALPHA_PREDICATE_def WF_PREDICATE_OVER_def H1_def)
+  apply (auto intro:unrest)
+done
+
+lift_definition AH2 :: 
+  "'a WF_ALPHA_PREDICATE \<Rightarrow> 
+   'a WF_ALPHA_PREDICATE"
+is "\<lambda> P. (\<alpha> P \<union>\<^sub>f \<lbrace>okay\<down>, okay\<down>\<acute>\<rbrace>, H2(\<pi> P))"
+  apply (simp add:WF_ALPHA_PREDICATE_def WF_PREDICATE_OVER_def H2_def)
+oops
+
 lemma REL_ALPHABET_in_alpha [closure]: "in\<^sub>\<alpha>a \<in> REL_ALPHABET"
   by (auto simp add:REL_ALPHABET_def var_defs)
 
-
 lemma REL_ALPHABET_out_alpha [closure]: "out\<^sub>\<alpha>a \<in> REL_ALPHABET"
   by (auto simp add:REL_ALPHABET_def var_defs)
-
 
 lemma DesignA_alphabet [alphabet]:
   "\<alpha> (P \<turnstile>\<^sub>\<alpha> Q) = \<alpha> P \<union>\<^sub>f \<alpha> Q \<union>\<^sub>f \<lbrace>okay\<down>, okay\<down>\<acute>\<rbrace>"
@@ -32,6 +65,25 @@ lemma DesignA_rel_closure [closure]:
   apply (simp add:WF_ALPHA_REL_def REL_ALPHABET_def alphabet)
   apply (simp add:closure)
 done
+
+lemma SkipDA_alphabet [alphabet]:
+  "a \<in> REL_ALPHABET \<Longrightarrow>
+   \<alpha>(II\<^bsub>D[a]\<^esub>) = a \<union>\<^sub>f \<lbrace>okay\<down>, okay\<down>\<acute>\<rbrace>"
+  by (auto simp add:SkipDA_def alphabet closure)
+
+lemma SkipDA_rel_closure [closure]:
+  "a \<in> REL_ALPHABET \<Longrightarrow> II\<^bsub>D[a]\<^esub> \<in> WF_ALPHA_REL"
+  apply (simp add:WF_ALPHA_REL_def REL_ALPHABET_def alphabet)
+  apply (simp add:closure)
+done
+
+lemma AH1_alphabet [alphabet]:
+  "\<alpha>(AH1(P)) = \<alpha> P \<union>\<^sub>f \<lbrace>okay\<down>, okay\<down>\<acute>\<rbrace>"
+  by (simp add:AH1.rep_eq pred_alphabet_def)
+
+lemma EvalA_AH1 [evala]:
+  "\<lbrakk>AH1(P)\<rbrakk>\<pi> = H1\<lbrakk>P\<rbrakk>\<pi>"
+  by (simp add:EvalA_def AH1.rep_eq)
 
 lemma WF_ALPHA_REL_EvalA_WF_RELATION [closure]:
   "P \<in> WF_ALPHA_REL \<Longrightarrow> \<lbrakk>P\<rbrakk>\<pi> \<in> WF_RELATION"
@@ -65,5 +117,159 @@ theorem DesignA_composition:
   apply (simp_all add:closure unrest)
   apply (auto)[1]
 done
+
+lemma AH1_DesignA:
+  assumes "okay\<down> \<notin>\<^sub>f \<alpha> P" "okay\<down>\<acute> \<notin>\<^sub>f \<alpha> P"
+          "okay\<down> \<notin>\<^sub>f \<alpha> Q" "okay\<down>\<acute> \<notin>\<^sub>f \<alpha> Q"
+  shows "AH1(P \<turnstile>\<^sub>\<alpha> Q) = P \<turnstile>\<^sub>\<alpha> Q"
+  by (utp_alpha_tac, utp_pred_auto_tac)
+
+lemma finsert_member [simp]: "x \<in>\<^sub>f xs \<Longrightarrow> finsert x xs = xs"
+  by auto
+
+lemma EvalR_ExprP'':
+  "\<lbrakk>ExprP e\<rbrakk>R = {(b1, b2). DestBool (\<lbrakk>e\<rbrakk>\<^sub>e (b1 \<oplus>\<^sub>b SS\<bullet>b2 on D\<^sub>1))
+                        \<and> b1 \<in> WF_REL_BINDING 
+                        \<and> b2 \<in> WF_REL_BINDING
+                        \<and> b1 \<cong> b2 on NON_REL_VAR}"
+  apply (auto simp add:evalr evale BindR_def urename RenameB_override_distr1 closure typing defined)
+  apply (metis RenameB_equiv_VAR_RENAME_ON_2 SS_VAR_RENAME_ON UNDASHED_DASHED_inter(16) binding_override_left_eq)
+  apply (rule_tac x="xa \<oplus>\<^sub>b SS\<bullet>y on D\<^sub>1" in exI)
+  apply (auto)
+  apply (metis WF_REL_BINDING_bc_DASHED_eq binding_override_equiv)
+  apply (simp add:urename RenameB_override_distr1 closure)
+  apply (metis (hide_lams, no_types) NON_REL_VAR_UNDASHED_DASHED SS_REL_VAR_overshadow WF_REL_BINDING_bc_DASHED_eq binding_equiv_override binding_override_assoc binding_override_minus binding_override_simps(2))
+done
+
+theorem undash_image_inter:
+  assumes "vs1 \<subseteq> DASHED" "vs2 \<subseteq> DASHED"
+  shows "undash ` (vs1 \<inter> vs2) = undash ` vs1 \<inter> undash ` vs2"
+  using assms
+  by (auto, metis IntI UnI1 Un_absorb1 dash_undash_DASHED imageI)
+
+(*
+theorem 
+  assumes
+  "P \<in> WF_RELATION" "Q \<in> WF_RELATION"
+  "VAR - vs1 \<sharp> P"
+  "VAR - vs2 \<sharp> Q"
+  "vs1 \<subseteq> vs2"
+  shows "P ; Q = P ; (\<exists>\<^sub>p vs2 - vs1. Q)"
+  apply (subgoal_tac "(\<exists>\<^sub>p vs2 - vs1 . Q) \<in> WF_RELATION")
+  apply (simp add:SemiR_algebraic_rel assms urename closure typing defined)
+*)
+
+theorem SkipRA_left_to_ExistsP:
+  assumes 
+    "p \<in> WF_RELATION" 
+    "HOMOGENEOUS vs2"
+    "vs2 \<subseteq> REL_VAR"
+    "vs1 \<subseteq> UNDASHED"
+    "out vs2 \<subseteq> dash ` vs1"
+    "UNDASHED - vs1 \<sharp> p"
+  shows "II\<^bsub>vs2\<^esub> ; p = (\<exists>\<^sub>p vs1 - in vs2. p)"
+  using assms
+  apply (subst SemiR_ExistsP_right[THEN sym, of _ _ "out vs2" "vs1"])
+  apply (simp_all add:unrest closure)
+  apply (auto intro:UNREST_subset unrest)[1]
+  apply (subst SemiR_SkipRA_left)
+  apply (simp_all add:unrest closure var_dist)
+  apply (rule unrest)
+  apply (rule UNREST_subset)
+  apply (simp)
+  apply (auto)[1]
+  apply (rule unrest)
+  apply (rule UNREST_subset)
+  apply (simp)
+  apply (auto)[1]
+done
+
+lemma WF_RELATION_REL_ALPHABET [closure]: 
+  "\<alpha> P \<in> REL_ALPHABET \<Longrightarrow> \<lbrakk>P\<rbrakk>\<pi> \<in> WF_RELATION"
+  by (auto intro:closure simp add:WF_ALPHA_REL_def)
+
+lemma [simp]: "a \<in> REL_ALPHABET \<Longrightarrow> (in\<^sub>\<alpha> a) \<union>\<^sub>f (out\<^sub>\<alpha> a) = a"
+  by (metis REL_ALPHABET_UNDASHED_DASHED alphabet_simps(14))
+
+thm SkipRA_closure
+
+lemma SkipRA_closure' [closure]:
+  "a \<in> REL_ALPHABET \<Longrightarrow> II\<^bsub>\<langle>a\<rangle>\<^sub>f\<^esub> \<in> WF_RELATION"
+  by (metis EvalA_SkipA SkipA_closure WF_ALPHA_REL_EvalA_WF_RELATION)
+ 
+lemma HOMOGENEOUS_HOM_ALPHA [closure]:
+  "a \<in> HOM_ALPHABET \<Longrightarrow> HOMOGENEOUS \<langle>a\<rangle>\<^sub>f"
+  by (metis (mono_tags) HOM_ALPHABET_def HOM_ALPHA_HOMOGENEOUS mem_Collect_eq)
+
+lemma WF_ALPHA_REL_REL_ALPHABET [closure]:
+  "\<alpha> P \<in> REL_ALPHABET \<Longrightarrow> P \<in> WF_ALPHA_REL"
+  by (simp add:WF_ALPHA_REL_def)
+
+lemma SkipD_SkipDA_link:
+  assumes 
+    "\<alpha> R \<in> DESIGN_ALPHABET" "\<alpha> R \<in> HOM_ALPHABET"
+  shows "II\<^sub>D ; \<lbrakk>R\<rbrakk>\<pi> = \<lbrakk>R\<rbrakk>\<pi> \<longleftrightarrow> (II\<^bsub>D[\<alpha> R]\<^esub> ;\<^sub>\<alpha> R = R)"
+proof -
+  have "II\<^sub>D ; \<lbrakk>R\<rbrakk>\<pi> = (true \<turnstile> II\<^bsub>\<langle>\<alpha> R -\<^sub>f \<lbrace>okay\<down>, okay\<down>\<acute>\<rbrace>\<rangle>\<^sub>f\<^esub>) ; \<lbrakk>R\<rbrakk>\<pi>"
+    apply (simp add:SkipD_def DesignD_def)
+    apply (subst BoolType_pvaux_cases[of "okay"])
+    apply (simp)
+    apply (subgoal_tac "HOMOGENEOUS (\<langle>\<alpha> R\<rangle>\<^sub>f)")
+    apply (simp add:usubst typing defined closure unrest assms)
+    apply (subst AndP_comm)
+    apply (subst SemiR_AndP_left_postcond)
+    apply (simp_all add: closure assms urename)
+    apply (subst AndP_comm) back
+    apply (subst SemiR_AndP_left_postcond)
+    apply (simp_all add: closure assms urename)
+    apply (metis (hide_lams, full_types) UNREST_SkipRA_NON_REL_VAR WF_RELATION_def mem_Collect_eq)
+    apply (subst SkipRA_left_to_ExistsP[of _ _ "D\<^sub>0"])
+    apply (simp_all add:closure var_dist unrest assms)
+    apply (subst SkipRA_left_to_ExistsP[of _ _ "in \<langle>\<alpha> R\<rangle>\<^sub>f"])
+    apply (insert assms)
+    apply (simp_all add:closure var_dist unrest)
+    apply (auto simp add:DESIGN_ALPHABET_def REL_ALPHABET_def)
+  done
+
+  also from assms have "in\<^sub>\<alpha> (\<alpha> R) \<union>\<^sub>f (in\<^sub>\<alpha> (\<alpha> R) -\<^sub>f \<lbrace>okay\<down>\<rbrace> \<union>\<^sub>f out\<^sub>\<alpha> (\<alpha> R)) = \<alpha> R" (is "?lhs = ?rhs")
+  proof -
+    have "?lhs = in\<^sub>\<alpha> (\<alpha> R) \<union>\<^sub>f out\<^sub>\<alpha> (\<alpha> R)"
+      by (auto)
+
+    thus ?thesis
+      by (simp add:closure assms)
+  qed
+
+  ultimately show ?thesis using assms
+    apply (simp add:SkipDA_def)
+    apply (utp_alpha_tac)
+    apply (simp add:alphabet_dist closure)
+  done
+qed
+
+declare [[coercion TautologyA]]
+
+theorem AH1_idem:
+  "AH1 (AH1 R) = AH1 R"
+  by (utp_alpha_tac, metis H1_idempotent)
+
+theorem AH1_monotone:
+  "P \<sqsubseteq> Q \<Longrightarrow> AH1 P \<sqsubseteq> AH1 Q"
+  apply (utp_alpha_tac)
+oops
+
+theorem AH1_algebraic:
+  assumes 
+    "\<alpha> R \<in> DESIGN_ALPHABET"
+    "\<alpha> R \<in> HOM_ALPHABET"
+  shows 
+    "((true\<^bsub>\<alpha> R\<^esub> ;\<^sub>\<alpha> R = true\<^bsub>\<alpha> R\<^esub>) \<and> (II\<^bsub>D[\<alpha> R]\<^esub> ;\<^sub>\<alpha> R = R)) \<longleftrightarrow> AH1(R) = R"
+  using assms
+  apply (simp add: SkipD_SkipDA_link[THEN sym] closure alphabet_dist)
+  apply (utp_alpha_tac)
+  apply (metis H1_algebraic HOM_ALPHABET_REL_ALPHABET Healthy_elim Healthy_intro WF_RELATION_REL_ALPHABET)
+done
+  
+
 
 end
